Add "kind" to ThreadEvent.t

src/drf/Lift.v
@@ -25,40 +25,32 @@ Require Import PIStep.
 Set Implicit Arguments.
 
 
-Definition TimeMap_lift (x: Loc.t) (t: Time.t) (tm: TimeMap.t) : TimeMap.t :=
-  fun y => if Loc.eq_dec x y then Time.join (tm y) t else tm y.
+Definition TimeMap_lift (l: Loc.t) (t: Time.t) (tm: TimeMap.t) : TimeMap.t :=
+  fun y => if Loc.eq_dec l y then Time.join (tm y) t else tm y.
 
-Definition Capability_lift (x: Loc.t) (t: Time.t) (rel: Capability.t) : Capability.t :=
+Definition Capability_lift (l: Loc.t) (t: Time.t) (rel: Capability.t) : Capability.t :=
   match rel with
   | Capability.mk ur rw sc => 
-    Capability.mk ur (TimeMap_lift x t rw) (TimeMap_lift x t sc)
+    Capability.mk ur (TimeMap_lift l t rw) (TimeMap_lift l t sc)
   end.
 
-Definition pi_step_lift_mem l t e M1 M2 : Prop :=
+Definition pi_step_lift_mem l t p e M1 M2 : Prop :=
   match ThreadEvent.is_writing e with
-  | Some (loc,from,to,val,rel,ord) =>
-    exists pm1 pm2 kind,
+  | Some (loc,from,to,val,rel,ord,kind) =>
+    <<NOTIN: Memory.get loc to p = None>> /\
+    exists pm1 pm2,
       <<PMREL: Memory.write pm1 M1 loc from to val (if Loc.eq_dec l loc then rel else Capability_lift l t rel) pm2 M2 kind>>
   | None =>
     M1 = M2
   end.
 
-Inductive pi_step_lift (l: Loc.t) (t: Time.t) : Ident.t -> ThreadEvent.t -> Configuration.t*Configuration.t*Memory.t ->  Configuration.t*Configuration.t*Memory.t -> Prop :=
-| pi_step_lift_intro tid e cS1 cS2 cT1 cT2 M1 M2
+Inductive pi_step_lift_except l t (tid_except:Ident.t): (Configuration.t*Configuration.t*Memory.t) -> (Configuration.t*Configuration.t*Memory.t) -> Prop :=
+| pi_step_lift_except_intro tid e cS1 cS2 cT1 cT2 M1 M2 lst lc
     (PI_STEP: pi_step true tid e (cS1,cT1) (cS2,cT2))
-    (MEM: pi_step_lift_mem l t e M1 M2):
-  pi_step_lift l t tid e (cS1,cT1,M1) (cS2,cT2,M2)
-.
-Hint Constructors pi_step_lift.
-
-Definition pi_step_lift_evt l t tid cSTM1 cSTM2 : Prop :=
-  step_union (pi_step_lift l t tid) cSTM1 cSTM2.
-Hint Unfold pi_step_lift_evt.
-
-Inductive pi_step_lift_except x t (tid_except:Ident.t) cSTM1 cSTM2: Prop :=
-| pi_step_lift_except_intro tid
-    (PI_STEP: pi_step_lift_evt x t tid cSTM1 cSTM2)
-    (TID: tid <> tid_except)
+    (FIND: IdentMap.find tid_except cT2.(Configuration.threads) = Some (lst,lc))
+    (MEM: pi_step_lift_mem l t lc.(Local.promises) e M1 M2)
+    (TID: tid <> tid_except):
+  pi_step_lift_except l t tid_except (cS1,cT1,M1) (cS2,cT2,M2)
 .
 Hint Constructors pi_step_lift_except.
 
@@ -73,10 +65,10 @@ Definition mem_eqlerel (m1 m2: Memory.t) : Prop :=
   <<LR: mem_sub Capability.le m1 m2>> /\
   <<RL: mem_sub (fun x y => Capability.le y x) m2 m1>>.
 
-Inductive mem_eqlerel_lift loc ts e (m1 m2: Memory.t) : Prop :=
+Inductive mem_eqlerel_lift l t p e (m1 m2: Memory.t) : Prop :=
 | mem_le_lift_intro m1'
   (MEMEQ: mem_eqlerel m1 m1')
-  (MEMWR: pi_step_lift_mem loc ts e m1' m2)
+  (MEMWR: pi_step_lift_mem l t p e m1' m2)
 .
 
 Definition conf_update_global (c: Configuration.t) sc (m: Memory.t) : Configuration.t :=
@@ -90,14 +82,13 @@ Inductive promises_aux tid cS cT loc ts : Prop :=
 .
 
 Lemma pi_steps_lift_except_pi_steps
-      cSTM1 cSTM2 x t tid
-      (STEPS: rtc (pi_step_lift_except x t tid) cSTM1 cSTM2):
+      cSTM1 cSTM2 l t tid
+      (STEPS: rtc (pi_step_lift_except l t tid) cSTM1 cSTM2):
   rtc (pi_step_except tid) cSTM1.(fst) cSTM2.(fst).
 Proof.
   induction STEPS; eauto.
   etrans; [|apply IHSTEPS].
-  inv H. inv PI_STEP. inv USTEP.
-  econs; eauto.
+  inv H. econs; eauto.
 Qed.
 
 Lemma pi_step_lifting
@@ -125,8 +116,8 @@ Proof.
 Admitted.
 
 Lemma rtc_pi_step_lift_except_find
-      cSTM1 cSTM2 tid loc ts
-      (STEPS: rtc (pi_step_lift_except loc ts tid) cSTM1 cSTM2):
+      cSTM1 cSTM2 tid l t
+      (STEPS: rtc (pi_step_lift_except l t tid) cSTM1 cSTM2):
   IdentMap.find tid cSTM1.(fst).(fst).(Configuration.threads) = IdentMap.find tid cSTM2.(fst).(fst).(Configuration.threads) /\
   IdentMap.find tid cSTM1.(fst).(snd).(Configuration.threads) = IdentMap.find tid cSTM2.(fst).(snd).(Configuration.threads).
 Proof.
@@ -138,9 +129,9 @@ Proof.
 Admitted. (* easy *)
 
 Lemma rtc_pi_step_except_local_wf
-      loc ts tid cS1 cT1 cSTM2
+      l t tid cS1 cT1 cSTM2
       (WF: pi_wf (cS1,cT1))
-      (STEPS_LIFT : rtc (pi_step_lift_except loc ts tid) (cS1, cT1, cT1.(Configuration.memory)) cSTM2):
+      (STEPS_LIFT : rtc (pi_step_lift_except l t tid) (cS1, cT1, cT1.(Configuration.memory)) cSTM2):
   pi_local_wf tid (promises_aux tid cSTM2.(fst).(fst) (conf_update_global cT1 cSTM2.(fst).(snd).(Configuration.sc) cSTM2.(snd)))
                   (cSTM2.(fst).(fst), conf_update_global cT1 cSTM2.(fst).(snd).(Configuration.sc) cSTM2.(snd)).
 Proof.
@@ -204,17 +195,15 @@ Proof.
 Admitted. (* ? *)
 
 Lemma pi_step_lift_mem_get
-      l t e m1 m1' m2 m2' loc ts from1 msg2 from2' msg2'
-      (LIFT1: pi_step_lift_mem l t e m1 m1')
-      (LIFT2: pi_step_lift_mem l t e m2 m2')
+      l t p1 p2 e m1 m1' m2 m2' loc ts from1 msg2 from2' msg2'
+      (LIFT1: pi_step_lift_mem l t p1 e m1 m1')
+      (LIFT2: pi_step_lift_mem l t p2 e m2 m2')
       (IN1: Memory.get loc ts m1 = Some (from1, msg2))
       (IN2: Memory.get loc ts m2' = Some (from2', msg2')):
   exists from2 msg2,
   Memory.get loc ts m2 = Some (from2, msg2).
 Proof.
-Admitted. (* wrong; gil *)
-
-
+Admitted. (* gil *)
 
 
 Lemma local_simul_fence
@@ -232,7 +221,7 @@ Lemma local_simul_write
   exists mS',
   Local.write_step (Local.mk com Memory.bot) sc mS loc from to val relr relw ord (Local.mk com' Memory.bot) sc' mS' kind.
 Proof.
-Admitted. (* wrong; closedness *)
+Admitted. (* closedness may be needed *)
 
 Lemma lift_fence
       sc1 sc2 sc2' com1 com2 com2' prm prm' ordr ordw
@@ -247,51 +236,50 @@ Proof.
 Admitted. (* jeehoon *)
 
 Lemma lift_write
-      com1 com2 com2' sc1 sc2 sc2' m1 m2 m2' prm prm' loc ts e loc' from to val relr1 relr2 relw2 ord kind
-      (LOCAL: Local.write_step (Local.mk com2 prm) sc2 m2 loc' from to val relr2 relw2 ord (Local.mk com2' prm') sc2' m2' kind)
+      com1 com2 com2' sc1 sc2 sc2' m1 m2 m2' prm prm' l t e loc from to val relr1 relr2 relw2 ord kind
+      (LOCAL: Local.write_step (Local.mk com2 prm) sc2 m2 loc from to val relr2 relw2 ord (Local.mk com2' prm') sc2' m2' kind)
       (CoMLE: Commit.le com1 com2)
       (SC: TimeMap.le sc1 sc2)
       (REL: Capability.le relr1 relr2)
-      (MEMLE: mem_eqlerel_lift loc ts e m1 m2):
+      (MEMLE: mem_eqlerel_lift l t prm e m1 m2):
   exists com1' sc1' m1' relw1,
-  <<LOCAL: Local.write_step (Local.mk com1 prm) sc1 m1 loc' from to val relr1 relw1 ord (Local.mk com1' prm') sc1' m1' kind>> /\
+  <<LOCAL: Local.write_step (Local.mk com1 prm) sc1 m1 loc from to val relr1 relw1 ord (Local.mk com1' prm') sc1' m1' kind>> /\
   <<CoMLE: Commit.le com1' com2'>> /\
   <<SC: TimeMap.le sc1' sc2'>> /\
-  <<MEMLE: mem_eqlerel_lift loc ts e m1' m2'>>.
+  <<MEMLE: mem_eqlerel_lift l t prm' e m1' m2'>>.
 Proof.
 Admitted. (* jeehoon *)
 
 Lemma lift_read
-      com1 com2 com2' m1 m2 prm prm' loc ts e loc' to val rel2 ordr
-      (LOCAL: Local.read_step (Local.mk com2 prm) m2 loc' to val rel2 ordr (Local.mk com2' prm'))
+      com1 com2 com2' m1 m2 prm l t e loc to val rel2 ordr
+      (LOCAL: Local.read_step (Local.mk com2 prm) m2 loc to val rel2 ordr (Local.mk com2' prm))
       (CoMLE: Commit.le com1 com2)
-      (MEMLE: mem_eqlerel_lift loc ts e m1 m2):
-  (exists from ordw,
-   <<EVENT: ThreadEvent.is_writing e = Some (loc', from, to, val, rel2, ordw)>>)
+      (MEMLE: mem_eqlerel_lift l t prm e m1 m2):
+  (exists from ordw kind,
+   <<EVENT: ThreadEvent.is_writing e = Some (loc, from, to, val, rel2, ordw, kind)>>)
   \/
   (exists com1' rel1,
-   <<LOCAL: Local.read_step (Local.mk com1 prm) m1 loc' to val rel1 ordr (Local.mk com1' prm')>> /\
+   <<LOCAL: Local.read_step (Local.mk com1 prm) m1 loc to val rel1 ordr (Local.mk com1' prm)>> /\
    <<CoMLE: Commit.le com1' com2'>>).
 Proof.
 Admitted. (* jeehoon *)
 
-
 Inductive thread_event_eqlerel: ThreadEvent.t -> ThreadEvent.t -> Prop :=
-| teel_promise loc from to val rel1 rel2
+| teel_promise loc from to val rel1 rel2 kind
     (LEREL: Capability.le rel1 rel2):
-  thread_event_eqlerel (ThreadEvent.promise loc from to val rel1) (ThreadEvent.promise loc from to val rel2) 
+  thread_event_eqlerel (ThreadEvent.promise loc from to val rel1 kind) (ThreadEvent.promise loc from to val rel2 kind) 
 | teel_silent:
   thread_event_eqlerel (ThreadEvent.silent) (ThreadEvent.silent)
 | teel_read loc ts val rel1 rel2 ord
     (LEREL: Capability.le rel1 rel2):
   thread_event_eqlerel (ThreadEvent.read loc ts val rel1 ord) (ThreadEvent.read loc ts val rel2 ord)
-| teel_write loc from to val rel1 rel2 ord
+| teel_write loc from to val rel1 rel2 ord kind
     (LEREL: Capability.le rel1 rel2):
-  thread_event_eqlerel (ThreadEvent.write loc from to val rel1 ord) (ThreadEvent.write loc from to val rel2 ord)
-| teel_update loc tsr tsw valr valw relr1 relr2 relw1 relw2 ordr ordw
+  thread_event_eqlerel (ThreadEvent.write loc from to val rel1 ord kind) (ThreadEvent.write loc from to val rel2 ord kind)
+| teel_update loc tsr tsw valr valw relr1 relr2 relw1 relw2 ordr ordw kind
     (LEREL: Capability.le relr1 relr2)
     (LEREL: Capability.le relw1 relw2):
-  thread_event_eqlerel (ThreadEvent.update loc tsr tsw valr valw relr1 relw1 ordr ordw) (ThreadEvent.update loc tsr tsw valr valw relr2 relw2 ordr ordw)
+  thread_event_eqlerel (ThreadEvent.update loc tsr tsw valr valw relr1 relw1 ordr ordw kind) (ThreadEvent.update loc tsr tsw valr valw relr2 relw2 ordr ordw kind)
 | teel_fence ordr ordw:
   thread_event_eqlerel (ThreadEvent.fence ordr ordw) (ThreadEvent.fence ordr ordw)
 | teel_syscall e:
@@ -306,11 +294,11 @@ Lemma lift_step
       (COM: Commit.le thS1.(Thread.local).(Local.commit) thT1.(Thread.local).(Local.commit))
       (PRM: thS1.(Thread.local).(Local.promises) = thT1.(Thread.local).(Local.promises))
       (SC: TimeMap.le thS1.(Thread.sc) thT1.(Thread.sc))
-      (MEM: mem_eqlerel_lift l t e thS1.(Thread.memory) thT1.(Thread.memory))
+      (MEM: mem_eqlerel_lift l t thT1.(Thread.local).(Local.promises) e thS1.(Thread.memory) thT1.(Thread.memory))
 : 
-  (exists loc ts from val relr relw ordr ordw,
+  (exists loc ts from val relr relw ordr ordw kind,
    <<EVTR: ThreadEvent.is_reading eT = Some (loc, ts, val, relr, ordr)>> /\
-   <<EVTW: ThreadEvent.is_writing e = Some (loc, from, ts, val, relw, ordw)>>)
+   <<EVTW: ThreadEvent.is_writing e = Some (loc, from, ts, val, relw, ordw, kind)>>)
   \/
   (exists eS thS2,
    <<EVT: thread_event_eqlerel eS eT>> /\
@@ -319,6 +307,6 @@ Lemma lift_step
    <<COM: Commit.le thS2.(Thread.local).(Local.commit) thT2.(Thread.local).(Local.commit)>> /\
    <<PRM: thS2.(Thread.local).(Local.promises) = thT2.(Thread.local).(Local.promises)>> /\
    <<SC: TimeMap.le thS2.(Thread.sc) thT2.(Thread.sc)>> /\
-   <<MEM: mem_eqlerel_lift l t e thS2.(Thread.memory) thT2.(Thread.memory)>>).
+   <<MEM: mem_eqlerel_lift l t thT2.(Thread.local).(Local.promises) e thS2.(Thread.memory) thT2.(Thread.memory)>>).
 Proof.
 Admitted. (* jeehoon *)
